\batchmode
\documentclass{article}
\usepackage{epsfig}
\pagestyle{empty}
\begin{document}
\[ h(t) = \frac{h_m}{2} \left[ 1 + cos( \frac{2\,\pi}{p} (t - d_m) ) \right] \]
\pagebreak

\[ G_{z}(r) = \frac{g}{\pi} \frac{(1-\nu ^2)}{E} \frac{1}{r} \]
\pagebreak

\[ G_{r}(r) = -\frac{g}{2\pi} \frac{(1+\nu)(1-2\nu)}{E} \frac{1}{r} \]
\pagebreak

$G_{z}(r)$
\pagebreak

$G_{r}(r)$
\pagebreak

$r$
\pagebreak

\[ U_{z,const} = \frac{g}{\pi} \frac{(1-\nu ^2)}{E} \]
\pagebreak

\[ U_{r, const} = -\frac{g}{2\pi} \frac{(1+\nu)(1-2\nu)}{E} \]
\pagebreak

\[ G_{z}^{H}(r) = G_{z,elastic}(r) + \frac{(1-\nu^2)g}{E\pi} \int^{\infty}_0{(\frac{B}{D} -1) J_0(\epsilon r)d\epsilon}\\ \]
\pagebreak

\[ G_{r}^{H}(r) = G_{r,elastic}(r) + \frac{g}{2\pi E (1-2\nu)} \int^{\infty}_0{\left[(1-\nu^2)(2\epsilon \frac{A}{D} + 4\nu)\right] J_1(\epsilon r)d\epsilon } \]
\pagebreak

$J_0$
\pagebreak

$J_1$
\pagebreak

$G_{z}^{H}(r)$
\pagebreak

$G_{r}^{H}(r)$
\pagebreak

$A, B,$
\pagebreak

$D$
\pagebreak

\[ A = \epsilon^2 H^2 - \nu (\cosh(2 \epsilon H) - 1) - \frac{2(1-\nu^2)}{E} g \rho_f (\nu \frac{\sinh(2 \epsilon H)}{\epsilon} + H)\\ \]
\pagebreak

\[ B = \frac{1}{2} \epsilon \sinh(2 \epsilon H) + \epsilon^2 H^2 + \frac{1-\nu^2}{E} g \rho_f (\cosh(2 \epsilon H) - 1) \]
\pagebreak

\[ D = -\epsilon^3 H^2 + \frac{1}{2} \epsilon (\cosh(2 \epsilon H) - 1) + \frac{1-\nu^2}{E} g \rho_f (\sinh(2 \epsilon H) + 2 \epsilon H) \]
\pagebreak

$H \to \infty$
\pagebreak

$\frac{A}{D} \to -\frac{2\nu}{\epsilon}$
\pagebreak

$\frac{A}{D} \to 1$
\pagebreak

$\[0 .. 0.003\]$
\pagebreak

\[ G_{r}^{H}(r) = G_{r,elastic}(r) - \frac{g}{2\pi E (1-2\nu)} \int^{\infty}_0{\left[(1-\nu^2)(2\epsilon \frac{A}{D} + 4\nu)\right] J_1(\epsilon r)d\epsilon } \]
\pagebreak

\end{document}
